

Leibniz-like Rule in Lie Groups

ATONU ROY CHOWDHURY

October 24, 2025; last updated December 1, 2025

§1 Background

Let M be a manifold, and $p \in M$. Then we have the notion of the tangent space $T_p M$ at the point p . This is the space of all point-derivations at p , i.e. all linear maps $X_p : C_p^\infty(M) \rightarrow \mathbb{R}$ such that

$$X_p(fg) = (X_p f)g(p) + f(p)(X_p g). \quad (1)$$

Here $C_p^\infty(M)$ is the germs of C^∞ functions $p \in M$, i.e. the set of equivalence classes of smooth functions that agree on some neighborhood of p . (1) can be thought of as the analogue of the Leibniz (product) rule for single-variable derivatives:

$$(fg)' = f'g + fg'. \quad (2)$$

Locally speaking, on a coordinate chart (U, x^1, \dots, x^n) around p , the tangent vector X_p is a linear combination of the partial derivatives

$$\left. \frac{\partial}{\partial x^1} \right|_p, \left. \frac{\partial}{\partial x^2} \right|_p, \dots, \left. \frac{\partial}{\partial x^n} \right|_p.$$

Now, given a smooth map $F : N \rightarrow M$ and $p \in N$, one can define the differential of F ,

$$\begin{aligned} (dF)_p : T_p N &\rightarrow T_{F(p)} M \\ [(dF)_p X_p] f &= X_p(f \circ F), \end{aligned} \quad (3)$$

for $f \in C_{F(p)}^\infty(M)$. Locally, $(dF)_p$ is the Jacobian matrix

$$\left[\frac{\partial F^i}{\partial x^j}(p) \right]_{1 \leq i \leq m, 1 \leq j \leq n}.$$

The alternate notation for $(dF)_p$ is $f_{*,p}$, which is also used in some literatures. But we will stick to the notation $(dF)_p$, since it manifests the fact that it's the differential of the smooth map F .

$(dF)_p$ takes us from a smooth map of $F : N \rightarrow M$ manifolds to a linear map $(dF)_p : T_p N \rightarrow T_{F(p)} M$ between vector spaces. So we can expect that it defines a functor from the category of

pointed manifolds to the category of vector spaces, given by

$$\begin{aligned} (M, p) &\mapsto T_p M \\ F : (N, p) \rightarrow (M, q) &\mapsto (dF)_p : T_p N \rightarrow T_{F(p)} M = T_q M. \end{aligned} \quad (4)$$

This, indeed, defines a functor since the differential has the following functorial property:

Theorem 1.1

Let $F : N \rightarrow M$ and $G : M \rightarrow P$ be smooth maps of manifolds, and $p \in N$. Then,

$$d(G \circ F)_p = (dG)_{F(p)} \circ (dF)_p. \quad (5)$$

In other words, the following diagram commutes:

$$\begin{array}{ccccc} T_p N & \xrightarrow{(dF)_p} & T_{F(p)} M & \xrightarrow{(dG)_{F(p)}} & T_{G(F(p))} P \\ & \searrow & & \nearrow & \\ & & d(G \circ F)_p = (dG)_{F(p)} \circ (dF)_p & & \end{array}$$

Furthermore, if $\mathbb{1}_M : M \rightarrow M$ is the identity map, then

$$(d\mathbb{1}_M)_p = \mathbb{1}_{T_p M} : T_p M \rightarrow T_p M. \quad (6)$$

We won't be proving it here, but the proof can be found in any elementary differential geometry textbook/course notes, for instance [here](#).

§2 Lie group setting

Now suppose the codomain of the smooth map is a Lie group G . Now, using the smooth multiplication in G , we can take the product of two smooth maps into G . In other words, given smooth maps $F_1, F_2 : N \rightarrow G$, we can consider the map

$$\begin{aligned} F_1 F_2 : N &\rightarrow G \\ p &\mapsto F_1(p) F_2(p). \end{aligned} \quad (7)$$

But then, naively, you may be prompted to write the differential $d(F_1 F_2)_p$ like this:

$$d(F_1 F_2)_p \stackrel{?}{=} (dF_1)_p F_2(p) + F_1(p) (dF_2)_p. \quad (8)$$

But if you look at it carefully, (8) makes no sense. $(dF_1)_p$ is a linear map $T_p N \rightarrow T_{F_1(p)} G$, and $F_2(p)$ is a Lie group element. How are we actually multiplying/composing them? Is there some sort of group action going on here? The same can be asked for $F_1(p)$ and $(dF_2)_p$ as well. But although (8) looks complete nonsense, there's a way to make sense of it. We can define the

left/right actions in such a way that (8) actually makes sense. Let

$$\begin{aligned} m : G \times G &\rightarrow G \\ (g_1, g_2) &\mapsto g_1 g_2 \end{aligned} \tag{9}$$

be the multiplication map on G , since G is a Lie group. Let L_g and R_g be the left and the multiplication by g , respectively. In other words,

$$\begin{aligned} L_g = m(g, -) : G &\rightarrow G \\ h &\mapsto gh; \end{aligned} \tag{10}$$

$$\begin{aligned} R_g = m(-, g) : G &\rightarrow G \\ h &\mapsto hg. \end{aligned} \tag{11}$$

The goal of this note is to prove the following:

Theorem 2.1

If G is a Lie group and $F_1, F_2 : N \rightarrow G$ are smooth maps, then

$$d(F_1 F_2)_p = (dR_{F_2(p)})_{F_1(p)} \circ (dF_1)_p + (dL_{F_1(p)})_{F_2(p)} \circ (dF_2)_p. \tag{12}$$

Note that the compositions make sense, because

$$T_p N \xrightarrow{(dF_1)_p} T_{F_1(p)} G \xrightarrow{(dR_{F_2(p)})_{F_1(p)}} T_{F_1(p)F_2(p)} G \tag{13}$$

$$T_p N \xrightarrow{(dF_2)_p} T_{F_2(p)} G \xrightarrow{(dL_{F_1(p)})_{F_2(p)}} T_{F_1(p)F_2(p)} G \tag{14}$$

Furthermore, the addition is also understood since we are adding two linear maps $T_p N \rightarrow T_{F_1(p)F_2(p)} G$.

§3 Proof

Throughout this section, we shall write $g = F_1(p)$ and $h = F_2(p)$.

Lemma 3.1

$$T_{(g,h)}(G \times G) \cong T_g G \times T_h G.$$

Proof. Consider the maps

$$G \xleftarrow{\pi_1} G \times G \xrightarrow{\pi_2} G \tag{15}$$

where $\pi_1(g_1, g_2) = g_1$ and $\pi_2(g_1, g_2) = g_2$. These are smooth maps. So we consider

$$T_g G \xleftarrow{(d\pi_1)_{(g,h)}} T_{(g,h)}(G \times G) \xrightarrow{(d\pi_2)_{(g,h)}} T_h G \quad (16)$$

Now we define

$$\begin{aligned} \Psi : T_{(g,h)}(G \times G) &\rightarrow T_g G \times T_h G \\ Z_{(g,h)} &\mapsto ((d\pi_1)_{(g,h)} Z_{(g,h)}, (d\pi_2)_{(g,h)} Z_{(g,h)}). \end{aligned} \quad (17)$$

In the other direction, we consider

$$G \xleftarrow{i_1} G \times G \xleftarrow{i_2} G \quad (18)$$

where $i_1(g_1) = (g_1, h)$ and $i_2(g_1) = (g, g_1)$. These are clearly smooth maps, since they are inclusions. Now,

$$T_g G \xrightarrow{(di_1)_g} T_{(g,h)}(G \times G) \xleftarrow{(di_2)_h} T_h G \quad (19)$$

Then we define

$$\begin{aligned} \Phi : T_g G \times T_h G &\rightarrow T_{(g,h)}(G \times G) \\ (X_g, Y_h) &\mapsto (di_1)_g X_g + (di_2)_h Y_h. \end{aligned} \quad (20)$$

Then one can check that both $\Psi \circ \Phi$ and $\Phi \circ \Psi$ are identity maps. The first one follows from the fact that $\pi_1 \circ i_1 = \pi_2 \circ i_2 = \text{id}_G$ so their differentials are also identity maps. The second one follows using a computation in local coordinates. \blacksquare

Proposition 3.2

Consider the smooth map $F = (F_1, F_2) : N \rightarrow G \times G$ defined by $p \mapsto (F_1(p), F_2(p))$. Then

$$(dF)_p = \left((dF_1)_p, (dF_2)_p \right), \quad (21)$$

under the identification $T_{(g,h)}(G \times G) \cong T_g G \times T_h G$. More concretely,

$$\Psi \circ (dF)_p = \left((dF_1)_p, (dF_2)_p \right). \quad (22)$$

Proof. Consider this commutative diagram in the category of smooth manifolds and smooth maps:

$$\begin{array}{ccccc} & & N & & \\ & \swarrow F_1 & \downarrow F & \searrow F_2 & \\ G & \xleftarrow{\pi_1} & G \times G & \xrightarrow{\pi_2} & G \end{array} \quad (23)$$

Then we have the following commutative diagram in the category of real vector spaces, by the functorial property of differential (Theorem 1.1):

$$\begin{array}{ccccc}
 & & T_p N & & \\
 & \swarrow (dF_1)_p & \downarrow (dF)_p & \searrow (dF_2)_p & \\
 T_g G & \xleftarrow{(d\pi_1)_{(g,h)}} & T_{(g,h)}(G \times G) & \xrightarrow{(d\pi_2)_{(g,h)}} & T_h G
 \end{array} \tag{24}$$

Now, given any $X_p \in T_p N$,

$$\begin{aligned}
 [\Psi \circ (dF)_p] X_p &= ((d\pi_1)_{(g,h)}(dF)_p X_p, (d\pi_2)_{(g,h)}(dF)_p X_p) \\
 &= ((dF_1)_p X_p, (dF_2)_p X_p),
 \end{aligned} \tag{25}$$

by the commutativity of (24). Therefore, $\Psi \circ (dF)_p = ((dF_1)_p, (dF_2)_p)$. \blacksquare

Proposition 3.3

For any $X_g \in T_g G$ and $Y_h \in T_h G$,

$$(dm)_{(g,h)} \circ \Phi(X_g, Y_h) = (dR_h)_g X_g + (dL_g)_h Y_h. \tag{26}$$

Proof. Consider this commutative diagram in the category of smooth manifolds and smooth maps:

$$\begin{array}{ccccc}
 G & \xrightarrow{i_1} & G \times G & \xleftarrow{i_2} & G \\
 & \searrow R_h = m \circ i_1 & \downarrow m & \swarrow L_g = m \circ i_2 & \\
 & & G & &
 \end{array} \tag{27}$$

Then we have the following commutative diagram in the category of real vector spaces, by the functorial property of differential (Theorem 1.1):

$$\begin{array}{ccccc}
 T_g G & \xrightarrow{(di_1)_g} & T_{(g,h)}(G \times G) & \xleftarrow{(di_2)_h} & T_h G \\
 & \searrow (dR_h)_g & \downarrow (dm)_{(g,h)} & \swarrow (dL_g)_h & \\
 & & T_{gh} G & &
 \end{array} \tag{28}$$

Now,

$$\begin{aligned}
(dm)_{(g,h)} \circ \Phi(X_g, Y_h) &= (dm)_{(g,h)} [(di_1)_g X_g + (di_2)_h Y_h] \\
&= (dm)_{(g,h)} (di_1)_g X_g + (dm)_{(g,h)} (di_2)_h Y_h \\
&= (dR_h)_g X_g + (dL_g)_h Y_h,
\end{aligned} \tag{29}$$

by the commutativity of (28). Therefore, $(dm)_{(g,h)} \circ \Phi(X_g, Y_h) = (dR_h)_g X_g + (dL_g)_h Y_h$. \blacksquare

Now we are ready to finally conclude the proof of Theorem 2.1.

Proof of Theorem 2.1. Note that

$$F_1 F_2 = m \circ (F_1, F_2) = m \circ F. \tag{30}$$

Therefore, by Theorem 1.1,

$$d(F_1 F_2)_p = (dm)_{gh} \circ (dF)_p. \tag{31}$$

$$\begin{array}{ccc}
& T_{(g,h)}(G \times G) & \\
(dF)_p \nearrow & \uparrow \Psi \quad \downarrow \Phi & \searrow (dm)_{(g,h)} \\
T_p N & & T_{gh} G \\
& T_g G \times T_h G &
\end{array} \tag{32}$$

Now, in light of (32), since $\Phi \circ \Psi$ is identity, we can conclude that

$$\begin{aligned}
d(F_1 F_2)_p &= (dm)_{gh} \circ (dF)_p = (dm)_{gh} \circ (\Phi \circ \Psi) \circ (dF)_p \\
&= (dm)_{gh} \circ \Phi \circ \left((dF_1)_p, (dF_2)_p \right)
\end{aligned} \tag{33}$$

$$= (dR_h)_g (dF_1)_p + (dL_g)_h (dF_2)_p. \tag{34}$$

Here (33) follows from Proposition 3.2 and (34) follows from Proposition 3.3. Hence, (12) is verified! \blacksquare

§4 Differential of the Multiplication and Inverse Maps

In Proposition 3.3, we have shown that the differential of the multiplication map is given by

$$(dm)_{(g,h)} \circ \Phi(X_g, Y_h) = (dR_h)_g X_g + (dL_g)_h Y_h. \tag{35}$$

As a special case, when $g = h = e$, we have $R_e = \text{id}_G$ and $L_e = \text{id}_G$, so that $(dR_e)_e = (dL_e)_e = \mathbb{1}_{T_e G}$. Therefore, we have the following corollary.

Corollary 4.1

The differential of the multiplication map at the identity is given by

$$(dm)_{(e,e)} \circ \Phi(X_g, Y_h) = X_g + Y_h. \quad (36)$$

Now, let's try to find the differential of the inverse map $i : G \rightarrow G$. $i \circ i = \text{id}_G$, so

$$(di)_{g^{-1}} \circ (di)_g = \mathbb{1}_{T_g G}. \quad (37)$$

Or, if we, for now, focus on the case $g = e$, we have

$$(di)_e \circ (di)_e = \mathbb{1}_{T_e G}. \quad (38)$$

So $(di)_e$ is an involution (i.e. squares to identity). However, it's not just any involution, as we'll see in the next result.

Proposition 4.2

Given $X_e \in T_e G$,

$$(di)_e X_e = -X_e. \quad (39)$$

In other words, $(di)_e = -\mathbb{1}_{T_e G}$.

Proof. We are going to use Theorem 2.1 to prove this. Here, $F_1 = \text{id}_G$, $F_2 = i$. Then $F_1 F_2 : G \rightarrow G$ is a constant map, so its differential is 0.

$$0 = d(F_1 F_2)_e = (dR_{F_2(e)})_{F_1(e)} \circ (dF_1)_e + (dL_{F_1(e)})_{F_2(e)} \circ (dF_2)_e. \quad (40)$$

Here, $F_1(e) = F_2(e) = e$, so we have $R_e = \text{id}_G$ and $L_e = \text{id}_G$, so that $(dR_e)_e = (dL_e)_e = \mathbb{1}_{T_e G}$. Therefore,

$$\begin{aligned} 0 &= (dF_1)_e + (dF_2)_e \\ &= (d \text{id}_G)_e + (di)_e \\ &= \mathbb{1}_{T_e G} + (di)_e \\ \implies (di)_e &= -\mathbb{1}_{T_e G}. \end{aligned} \quad (41)$$

■

Corollary 4.3

Given any $g \in G$,

$$(di)_g = - (dR_{g^{-1}})_e (dL_{g^{-1}})_g. \quad (42)$$

Proof. First, note that

$$i = R_{g^{-1}} \circ i \circ L_{g^{-1}}. \quad (43)$$

Indeed, the RHS evaluated at $x \in G$ gives us

$$\begin{aligned} R_{g^{-1}} \circ i \circ L_{g^{-1}}(x) &= R_{g^{-1}} \circ i(g^{-1}x) \\ &= (g^{-1}x)^{-1} g^{-1} \\ &= (x^{-1}g) g^{-1} \\ &= x^{-1}. \end{aligned} \quad (44)$$

Now using chain rule on (43), we have

$$(di)_g = (dR_{g^{-1}})_e (di)_e (dL_{g^{-1}})_g = - (dR_{g^{-1}})_e (dL_{g^{-1}})_g, \quad (45)$$

since $(di)_e = -\mathbb{1}_{T_e G}$. ■